skip_list/spec/insert.v
@@ -18,284 +18,54 @@ Module AddSpec (Params: SKIP_LIST_PARAMS).
   Section Proofs.
     Context `{!heapGS Σ, !gset_list_unionGS Σ, !lockG Σ} (lvlN : namespace).
 
-    Theorem tryInsert_spec (curr head: node_rep) (key: Z) 
-      (q: frac) (Skeys: gset Z) (bot: lazy_gname) :
+    Theorem linkNode_spec (head pred succ: node_rep) (key: Z)
+      (q: frac) (Skeys: gset Z) (Γ: lazy_gname) (obot: option lazy_gname) 
+      (l: loc) (γ: gname) (odown: option loc) :
       INT_MIN < key < INT_MAX →
-      {{{
-        is_lazy_list lvlN head q Skeys bot from_bot_list
+      {{{ 
+        is_lazy_list lvlN head q Skeys Γ (from_bot_list obot)
         ∗
-        (⌜ curr = head ⌝ ∨ own (s_auth bot) (◯ {[ curr ]}))
+        (⌜ pred = head ⌝ ∨ own (s_auth Γ) (◯ {[ pred ]}))
         ∗
-        ⌜ node_key curr < key ⌝
+        ⌜ node_key pred < key < node_key succ ⌝
+        ∗
+        ⌜ node_next pred = Some l ⌝
+        ∗
+        is_lock γ (node_lock pred) (node_inv l)
+        ∗
+        l ↦{#1 / 2} rep_to_node succ
+        ∗
+        locked γ
+        ∗
+        from_bot_list obot key odown
       }}}
-        tryInsert (rep_to_node curr) #key
-      {{{ v new, RET v;
-        is_lazy_list lvlN head q (Skeys ∪ {[ key ]}) bot from_bot_list
-        ∗
-        ( 
-          ⌜ v = NONEV ⌝ ∨ 
-          ( 
-            ⌜ v = SOMEV (rep_to_node new) ⌝ 
-            ∗ 
-            ⌜ node_key new = key ⌝
-            ∗ 
-            own (s_auth bot) (◯ {[ new ]})
-            ∗ 
-            own (s_toks bot) (GSet {[ node_key new ]})
-          )
-        )
-      }}}.
-    Proof.
-      iIntros (Hkey_range Φ) "(Hlazy & #Hown_curr & %Hrange) HΦ".
-      iDestruct "Hlazy" as (Sfrag) "(%Hequiv & Hown_frag & #Hinv)".
-      wp_lam. wp_let.
-
-      wp_apply findLock_spec.
-      { iFrame "#". iPureIntro; lia. }
-      iIntros (pred succ) "(%Hrange' & #Hown_pred & #Hown_succ & Hlock)".
-      iDestruct "Hlock" as (l γ) "(%Hsome & #Hlock & Hpt & Hlocked)".
-
-      wp_pures. wp_lam. wp_pures.
-      case_bool_decide as Hcase; wp_if.
-      + assert (key = node_key succ) as Heq by congruence.
-        iDestruct "Hown_succ" as "[Hown_succ|%Hsucc]"; last first.
-        { subst; exfalso. rewrite /node_key/tail/= in Hkey_range; lia. }
-
-        wp_lam. wp_bind (Snd _).
-        iInv lvlN as (S Skeys' L) "(>%Hperm & >%Hsort &>%Hequiv' & >Hown_auth & >Hown_frac & >Hown_toks & Hlist)" "Hclose".
-        iDestruct (own_valid_2 with "Hown_auth Hown_succ") 
-          as %[Hvalid%gset_included]%auth_both_valid_discrete.
-        iDestruct (own_valid_2 with "Hown_frac Hown_frag") 
-          as %Hsub%frac_auth_included_total%gset_included.
-        iMod (own_update_2 with "Hown_frac Hown_frag") as "[Hown_frac Hown_frag]".
-        { apply frac_auth_update, (gset_local_update_union _ _ {[ succ ]}). }
-
-        wp_proj.
-        iMod ("Hclose" with "[Hlist Hown_auth Hown_frac Hown_toks]") as "_".
-        {
-          iNext; iExists S, Skeys', L.
-          assert (S = S ∪ {[ succ ]}) as <- by set_solver.
-          by iFrame.
-        }
-        iModIntro.
-
-        wp_apply (release_spec with "[Hlock Hpt Hlocked]"); first done.
-        { iFrame "# ∗"; iExists succ; iFrame. }
-        iIntros "_". wp_pures.
-        iModIntro. iApply ("HΦ" $! _ succ).
-        iSplitR ""; last by iLeft.
-        iExists (Sfrag ∪ {[ succ ]}). 
-        iFrame "# ∗". iPureIntro.
-
-        eapply key_equiv_union.
-        { done. }
-        { by do 2 apply node_rep_sorted_app in Hsort as [? Hsort]. }
-        { done. }
-        { rewrite Heq /key_equiv ?elements_singleton //. }
-        { by apply union_subseteq. }
-      + wp_lam. wp_pures.
-        rewrite Hsome; wp_match.
-        wp_load. wp_let. wp_alloc l' as "Hpt'". wp_let.
-        iDestruct "Hpt'" as "(Hpt' & Hpt'_dup)".
-        
-        wp_apply (newlock_spec (node_inv l') with "[Hpt'_dup]").
-        { iExists succ; iFrame. }
-        iIntros (lk) "#Hlock'". iDestruct "Hlock'" as (γ') "Hlock'".
-
-        wp_pures.
-        rewrite (fold_rep_to_node (key, Some l', None, lk)).
-        set (new := (key, Some l', None, lk)).
-        
-        wp_bind (Store _ _).
-        iInv lvlN as (S Skeys' L) "(>%Hperm & >%Hsort & >%Hequiv' & >Hown_auth & >Hown_frac & >Hown_toks & Hlist)" "Hclose".
-
-        iAssert ⌜ pred = head ∨ In pred L ⌝%I
-          with "[Hown_auth Hown_pred]" as %Hpred_range.
-        {
-          iDestruct "Hown_pred" as "[Heq|Hown]"; first by iLeft.
-          iDestruct (own_valid_2 with "Hown_auth Hown") 
-            as %[Hvalid%gset_included]%auth_both_valid_discrete.
-          iPureIntro; right. 
-          rewrite -elem_of_list_In Hperm elem_of_elements.
-          set_solver.
-        }
-
-        assert (key ≠ node_key succ) as Hneq by congruence.
-        rewrite (list_equiv_insert head pred new succ L l l' γ'); first last.
-        { done. }
-        { auto. }
-        { assert (node_key new = key) as -> by auto; lia. }
-        { rewrite /node_key/=; lia. }
-
-        iDestruct ("Hlist" with "[Hpt Hpt' Hlock]") as "Hlist".
-        { iNext; by iFrame "# ∗". }
-        iDestruct "Hlist" as (L' L1 L2) "(Hpt & >%Hsplit & >%Hsort' & >%Hperm' & Himp)".
-
-        iDestruct (own_valid_2 with "Hown_frac Hown_frag") 
-          as %HsubS%frac_auth_included_total%gset_included.
-
-        assert (key ∉ Skeys') as Hnin'.
-        {
-          intros Hfalse.
-          rewrite -elem_of_elements Hequiv' elem_of_list_In -Hperm in_map_iff in Hfalse.
-          destruct Hfalse as [x [Hkey Hin]].
-          
-          apply (sorted_node_lt_nin L1 L2 pred succ x).
-          { rewrite -Hsplit //. }
-          { rewrite Hkey; lia. }
-          rewrite -Hsplit. apply in_or_app; right. apply in_or_app; by left.
-        }
-
-        assert (key ∉ Skeys) as Hnin.
-        {
-          intros Hfalse.
-          rewrite -elem_of_elements Hequiv elem_of_list_In in_map_iff in Hfalse.
-          destruct Hfalse as [x [Hkey Hin]].
-          rewrite -elem_of_list_In elem_of_elements in Hin.
-          assert (x ∈ S) as HinS by set_solver; clear Hin.
-          rewrite -elem_of_elements -Hperm elem_of_list_In in HinS.
-          
-          apply (sorted_node_lt_nin L1 L2 pred succ x).
-          { rewrite -Hsplit //. }
-          { rewrite Hkey; lia. }
-          rewrite -Hsplit. apply in_or_app; right. apply in_or_app; by left.
-        }
-
-        iMod (own_update with "Hown_auth") as "[Hown_auth Hown_auth_frag]".
-        { apply auth_update_alloc, (gset_local_update_union _ _ {[ new ]}). }
-        assert (ε ∪ {[ new ]} = {[ new ]}) as -> by set_solver.
-
-        iMod (own_update_2 with "Hown_frac Hown_frag") as "[Hown_frac Hown_frac_frag]".
-        { apply frac_auth_update, (gset_local_update_union _ _ {[ new ]}). }
-
-        rewrite (gset_union_diff key); first last.
-        { done. }
-        { rewrite Zlt_range_spec; lia. }
-        rewrite -gset_disj_union; last set_solver.
-        iDestruct "Hown_toks" as "(Hown_toks & Hown_tok)".
-        
-        wp_store.
-        iDestruct "Hpt" as "(Hpt & Hpt_dup)".
-        iPoseProof ("Himp" with "Hpt_dup") as "Hlist".
-        iMod ("Hclose" with "[Hlist Hown_auth Hown_frac Hown_toks]") as "_".
-        {
-          iNext; iExists (S ∪ {[ new ]}), (Skeys' ∪ {[ key ]}), L'.
-          iFrame. iSplit; last first. iSplit; first done.
-          by (iPureIntro; apply key_equiv_insert_nin).
-          
-          iPureIntro.
-          apply NoDup_Permutation.
-          { 
-            apply node_rep_sorted_app in Hsort'; destruct Hsort' as [_ Hsort']. 
-            apply node_rep_sorted_app in Hsort'; destruct Hsort' as [Hsort' _].
-            by apply sorted_node_lt_no_dup.
-          } 
-          { apply NoDup_elements. }
-
-          simpl in Hperm'; apply Permutation_cons_inv in Hperm'.
-          intros x; split.
-          - rewrite elem_of_elements Hperm' elem_of_list_In.
-            intros Hin. destruct Hin as [Heq|Hin].
-            * set_solver.
-            * apply elem_of_union_l. 
-              by rewrite -elem_of_elements -Hperm elem_of_list_In.
-          - rewrite elem_of_elements Hperm'. 
-            intros Hin. apply elem_of_union in Hin as [Hin|Heq].
-            * rewrite elem_of_list_In. right.
-              by rewrite -elem_of_list_In Hperm elem_of_elements.
-            * set_solver.
-        }
-
-        iModIntro. wp_pures. wp_lam. wp_pures.
-        wp_apply (release_spec with "[Hlock Hpt Hlocked]"); first done.
-        { iFrame "# ∗"; iExists new; iFrame. }
-        iIntros "_". wp_pures. 
-        iModIntro. iApply "HΦ".
-        iSplitR "Hown_tok Hown_auth_frag"; last by (iRight; iFrame).
-        iExists (Sfrag ∪ {[ new ]}).
-        iFrame "# ∗". iPureIntro.
-        apply key_equiv_insert_nin; auto.
-    Qed.
-
-    Theorem insert_spec (curr down head: node_rep) (key: Z) 
-      (q: frac) (Stop Sbot: gset Z) (top bot: lazy_gname) :
-      INT_MIN < key < INT_MAX →
-      {{{
-        is_lazy_list lvlN head q Stop top (from_sub_list bot)
-        ∗
-        (⌜ curr = head ⌝ ∨ own (s_auth top) (◯ {[ curr ]}))
-        ∗
-        ⌜ node_key curr < key ⌝
+        linkNode (rep_to_node pred) #key (oloc_to_val odown)
+      {{{ new, RET SOMEV (rep_to_node new);
+        is_lazy_list lvlN head q (Skeys ∪ {[ key ]}) Γ (from_bot_list obot)
         ∗ 
-        ⌜ node_key down = key ⌝
+        own (s_auth Γ) (◯ {[ new ]})
         ∗ 
-        own (s_auth bot) (◯ {[ down ]})
-        ∗ 
-        own (s_toks bot) (GSet {[ node_key down ]})
-      }}}
-        insert (rep_to_node curr) #key (rep_to_node down)
-      {{{ v new, RET v;
-        is_lazy_list lvlN head q (Stop ∪ {[ key ]}) top (from_sub_list bot)
-        ∗
-        ⌜ v = SOMEV (rep_to_node new) ⌝ 
+        own (s_toks Γ) (GSet {[ node_key new ]})
         ∗ 
         ⌜ node_key new = key ⌝
-        ∗ 
-        own (s_auth top) (◯ {[ new ]})
-        ∗ 
-        own (s_toks top) (GSet {[ node_key new ]})
       }}}.
     Proof.
-      iIntros (Hkey_range Φ) "(Hlazy & #Hown_curr & %Hrange & %Hdown & #Hown_down & Hown_tok) HΦ".
+      iIntros (Hkey_range Φ) "(Hlazy & #Hown_pred & %Hrange & %Hpred_next & #Hlock & Hpt & Hlocked & HP) HΦ".
       iDestruct "Hlazy" as (Sfrag) "(%Hequiv & Hown_frag & #Hinv)".
-      wp_lam. wp_let. wp_let.
 
-      wp_apply findLock_spec.
-      { iFrame "#". iPureIntro; lia. }
-      iIntros (pred succ) "(%Hrange' & #Hown_pred & #Hown_succ & Hlock)".
-      iDestruct "Hlock" as (l γ) "(%Hsome & #Hlock & Hpt & Hlocked)".
-
-      wp_pures. wp_lam. wp_pures.
-      rewrite Hsome; wp_match.
+      wp_lam. wp_pures. 
+      wp_lam. wp_pures.
+      rewrite Hpred_next; wp_match.
       wp_load. wp_let. 
       wp_alloc l' as "Hpt'". wp_let.
-      wp_alloc l'' as "Hpt''". wp_let.
       iDestruct "Hpt'" as "(Hpt' & Hpt'_dup)".
       
       wp_apply (newlock_spec (node_inv l') with "[Hpt'_dup]").
       { iExists succ; iFrame. }
       iIntros (lk) "#Hlock'". iDestruct "Hlock'" as (γ') "Hlock'".
 
-      wp_bind (InjR _).
-      iInv lvlN as (S Skeys' L) "(>%Hperm & >%Hsort & >%Hequiv' & Hown_auth & Hown_frac & Hown_toks & Hlist)" "Hclose".
-      wp_inj.
-
-      iAssert ⌜ key ≠ node_key succ ⌝%I
-        with "[Hown_auth Hown_succ Hown_tok Hlist]" as %Hneq.
-      {
-        iDestruct "Hown_succ" as "[Hown|%Heq]"; last first.
-        { iPureIntro; rewrite Heq /node_key /=; lia. } 
-
-        iDestruct (own_valid_2 with "Hown_auth Hown") 
-          as %[Hvalid%gset_included]%auth_both_valid_discrete.
-        assert (succ ∈ S) by set_solver.
-
-        rewrite list_equiv_invert_L; last first.
-        { by rewrite -elem_of_list_In Hperm elem_of_elements. }
-        iDestruct "Hlist" as (? ? ? ? ? ) "(_ & _ & _ & _ & _ & HP & _)".
-        iDestruct "HP" as (? ?) "(_ & _ & _ & Hown_tok' & %Hsucc)".
-
-        iDestruct (own_valid_2 with "Hown_tok Hown_tok'") as 
-          %Hdisj%gset_disj_valid_op.
-        iPureIntro; set_solver.
-      }
-
-      iMod ("Hclose" with "[Hlist Hown_auth Hown_frac Hown_toks]") as "_".
-      { iNext; iExists S, Skeys', L; by iFrame "# ∗". }
-      clear Hperm Hsort Hequiv' S Skeys' L.
-
-      iModIntro; wp_pures.
-      set (new := (key, Some l', Some l'', lk)).
+      wp_pures.
+      set (new := (key, Some l', odown, lk)).
       rewrite (fold_rep_to_node new).
       
       wp_bind (Store _ _).
@@ -318,12 +88,8 @@ Module AddSpec (Params: SKIP_LIST_PARAMS).
       { assert (node_key new = key) as -> by auto; lia. }
       { rewrite /node_key/=; lia. }
 
-      iDestruct ("Hlist" with "[Hpt Hpt' Hpt'' Hlock Hown_tok]") as "Hlist".
-      { 
-        iNext; iFrame "# ∗". 
-        iSplit; first done. iSplit; first done.
-        iExists l'', down. by iFrame "# ∗".
-      }
+      iDestruct ("Hlist" with "[Hpt Hpt' Hlock HP]") as "Hlist".
+      { iNext; by iFrame "# ∗". }
       iDestruct "Hlist" as (L' L1 L2) "(Hpt & >%Hsplit & >%Hsort' & >%Hperm' & Himp)".
 
       iDestruct (own_valid_2 with "Hown_frac Hown_frag") 
@@ -341,7 +107,7 @@ Module AddSpec (Params: SKIP_LIST_PARAMS).
         rewrite -Hsplit. apply in_or_app; right. apply in_or_app; by left.
       }
 
-      assert (key ∉ Stop) as Hnin.
+      assert (key ∉ Skeys) as Hnin.
       {
         intros Hfalse.
         rewrite -elem_of_elements Hequiv elem_of_list_In in_map_iff in Hfalse.
@@ -410,6 +176,180 @@ Module AddSpec (Params: SKIP_LIST_PARAMS).
       iExists (Sfrag ∪ {[ new ]}).
       iFrame "# ∗". iPureIntro.
       apply key_equiv_insert_nin; auto.
+    Qed.
+
+    Theorem tryInsert_spec (curr head: node_rep) (key: Z) 
+      (q: frac) (Skeys: gset Z) (bot: lazy_gname) :
+      INT_MIN < key < INT_MAX →
+      {{{
+        is_lazy_list lvlN head q Skeys bot (from_bot_list None)
+        ∗
+        (⌜ curr = head ⌝ ∨ own (s_auth bot) (◯ {[ curr ]}))
+        ∗
+        ⌜ node_key curr < key ⌝
+      }}}
+        tryInsert (rep_to_node curr) #key
+      {{{ v new, RET v;
+        is_lazy_list lvlN head q (Skeys ∪ {[ key ]}) bot (from_bot_list None)
+        ∗
+        ( 
+          ⌜ v = NONEV ⌝ ∨ 
+          ( 
+            ⌜ v = SOMEV (rep_to_node new) ⌝ 
+            ∗ 
+            own (s_auth bot) (◯ {[ new ]})
+            ∗ 
+            own (s_toks bot) (GSet {[ node_key new ]})
+            ∗ 
+            ⌜ node_key new = key ⌝
+          )
+        )
+      }}}.
+    Proof.
+      iIntros (Hkey_range Φ) "(Hlazy & #Hown_curr & %Hrange) HΦ".
+      iDestruct "Hlazy" as (Sfrag) "(%Hequiv & Hown_frag & #Hinv)".
+      wp_lam. wp_let.
+
+      wp_apply findLock_spec.
+      { iFrame "#". iPureIntro; lia. }
+      iIntros (pred succ) "(%Hrange' & #Hown_pred & #Hown_succ & Hlock)".
+      iDestruct "Hlock" as (l γ) "(%Hsome & #Hlock & Hpt & Hlocked)".
+
+      wp_pures. wp_lam. wp_pures.
+      case_bool_decide as Hcase; wp_if.
+      + assert (key = node_key succ) as Heq by congruence.
+        iDestruct "Hown_succ" as "[Hown_succ|%Hsucc]"; last first.
+        { subst; exfalso. rewrite /node_key/tail/= in Hkey_range; lia. }
+
+        wp_lam. wp_bind (Snd _).
+        iInv lvlN as (S Skeys' L) "(>%Hperm & >%Hsort &>%Hequiv' & >Hown_auth & >Hown_frac & >Hown_toks & Hlist)" "Hclose".
+        iDestruct (own_valid_2 with "Hown_auth Hown_succ") 
+          as %[Hvalid%gset_included]%auth_both_valid_discrete.
+        iDestruct (own_valid_2 with "Hown_frac Hown_frag") 
+          as %Hsub%frac_auth_included_total%gset_included.
+        iMod (own_update_2 with "Hown_frac Hown_frag") as "[Hown_frac Hown_frag]".
+        { apply frac_auth_update, (gset_local_update_union _ _ {[ succ ]}). }
+
+        wp_proj.
+        iMod ("Hclose" with "[Hlist Hown_auth Hown_frac Hown_toks]") as "_".
+        {
+          iNext; iExists S, Skeys', L.
+          assert (S = S ∪ {[ succ ]}) as <- by set_solver.
+          by iFrame.
+        }
+        iModIntro.
+
+        wp_apply (release_spec with "[Hlock Hpt Hlocked]"); first done.
+        { iFrame "# ∗"; iExists succ; iFrame. }
+        iIntros "_". wp_pures.
+        iModIntro. iApply ("HΦ" $! _ succ).
+        iSplitR ""; last by iLeft.
+        iExists (Sfrag ∪ {[ succ ]}). 
+        iFrame "# ∗". iPureIntro.
+
+        eapply key_equiv_union.
+        { done. }
+        { by do 2 apply node_rep_sorted_app in Hsort as [? Hsort]. }
+        { done. }
+        { rewrite Heq /key_equiv ?elements_singleton //. }
+        { by apply union_subseteq. }
+      + assert (key ≠ node_key succ) as Hneq by congruence.
+        assert (oloc_to_val None = NONEV) as <- by auto.
+
+        wp_apply (linkNode_spec with "[Hpt Hlocked Hown_frag]").
+        { done. }
+        { 
+          iFrame "# ∗". 
+          iSplit. iExists Sfrag; by iFrame.
+          iPureIntro. by split; first lia.
+        }
+        
+        iIntros (new) "(Hlazy & Hkey & Hown_frag & Hown_tok)".
+        iApply "HΦ". iSplitL "Hlazy"; last iRight; by iFrame.
+    Qed.
+
+    Theorem insert_spec (curr down head: node_rep) (key: Z) 
+      (q: frac) (Stop Sbot: gset Z) (top bot: lazy_gname) :
+      INT_MIN < key < INT_MAX →
+      {{{
+        is_lazy_list lvlN head q Stop top (from_bot_list (Some bot))
+        ∗
+        (⌜ curr = head ⌝ ∨ own (s_auth top) (◯ {[ curr ]}))
+        ∗
+        ⌜ node_key curr < key ⌝
+        ∗ 
+        own (s_auth bot) (◯ {[ down ]})
+        ∗ 
+        own (s_toks bot) (GSet {[ node_key down ]})
+        ∗ 
+        ⌜ node_key down = key ⌝
+      }}}
+        insert (rep_to_node curr) #key (rep_to_node down)
+      {{{ new, RET SOMEV (rep_to_node new);
+        is_lazy_list lvlN head q (Stop ∪ {[ key ]}) top (from_bot_list (Some bot))
+        ∗ 
+        own (s_auth top) (◯ {[ new ]})
+        ∗ 
+        own (s_toks top) (GSet {[ node_key new ]})
+        ∗ 
+        ⌜ node_key new = key ⌝
+      }}}.
+    Proof.
+      iIntros (Hkey_range Φ) "(Hlazy & #Hown_curr & %Hrange & #Hown_down & Hown_tok & %Hdown) HΦ".
+      iDestruct "Hlazy" as (Sfrag) "(%Hequiv & Hown_frag & #Hinv)".
+      wp_lam. wp_let. wp_let.
+
+      wp_apply findLock_spec.
+      { iFrame "#". iPureIntro; lia. }
+      iIntros (pred succ) "(%Hrange' & #Hown_pred & #Hown_succ & Hlock)".
+      iDestruct "Hlock" as (l γ) "(%Hsome & #Hlock & Hpt & Hlocked)".
+
+      wp_let. wp_match.
+      wp_bind (Fst _).
+      iInv lvlN as (S Skeys' L) "(>%Hperm & >%Hsort & >%Hequiv' & Hown_auth & Hown_frac & Hown_toks & Hlist)" "Hclose".
+      wp_proj.
+
+      iAssert ⌜ key ≠ node_key succ ⌝%I
+        with "[Hown_auth Hown_succ Hown_tok Hlist]" as %Hneq.
+      {
+        iDestruct "Hown_succ" as "[Hown|%Heq]"; last first.
+        { iPureIntro; rewrite Heq /node_key /=; lia. } 
+
+        iDestruct (own_valid_2 with "Hown_auth Hown") 
+          as %[Hvalid%gset_included]%auth_both_valid_discrete.
+        assert (succ ∈ S) by set_solver.
+
+        rewrite list_equiv_invert_L; last first.
+        { by rewrite -elem_of_list_In Hperm elem_of_elements. }
+        iDestruct "Hlist" as (? ? ? ? ? ) "(_ & _ & _ & _ & _ & HP & _)".
+        destruct (node_down succ) as [d|]; last by iExFalso.
+        iDestruct "HP" as (?) "(_ & _ & Hown_tok' & %Hsucc)".
+
+        iDestruct (own_valid_2 with "Hown_tok Hown_tok'") as 
+          %Hdisj%gset_disj_valid_op.
+        iPureIntro; set_solver.
+      }
+
+      iMod ("Hclose" with "[Hlist Hown_auth Hown_frac Hown_toks]") as "_".
+      { iNext; iExists S, Skeys', L; by iFrame "# ∗". }
+
+      iModIntro; wp_pures. 
+      wp_alloc d as "Hpt_down". 
+      wp_pures.
+
+      assert (oloc_to_val (Some d) = SOMEV #d) as <- by auto.
+      iAssert (from_bot_list (Some bot) key (Some d)) 
+        with "[Hpt_down Hown_tok]" as "HP".
+      { iExists down; by iFrame "# ∗". }
+
+      wp_apply (linkNode_spec with "[Hpt Hlocked Hown_frag HP]").
+      { done. }
+      { 
+        iFrame "# ∗". 
+        iSplit. iExists Sfrag; by iFrame.
+        iPureIntro. by split; first lia.
+      }
+      iApply "HΦ".
     Qed.
 
   End Proofs.
